devel/Iron/Language/SystemF2Effect/Store.v
@@ -1,14 +1,15 @@
 
+Require Import Iron.Language.SystemF2Effect.KiJudge.
 Require Import Iron.Language.SystemF2Effect.Ty.
 Require Import Iron.Language.SystemF2Effect.TyJudge.
-Require Import Iron.Language.SystemF2Effect.VaExpBase.
+Require Import Iron.Language.SystemF2Effect.Va.
+Require Export Iron.Language.SystemF2Effect.StoreBind.
 
 
-(********************************************************************)
-Definition store := list val.
+(* A store is a list of store bindings. *)
+Definition store := list sbind.
 
 
-(********************************************************************)
 (* Store typing models the store.
    All types in the store typing have a corresponding binding in
    the store *)
@@ -17,30 +18,16 @@ Definition STOREM (se: stenv) (ss: store)
 Hint Unfold STOREM.
 
 
-(********************************************************************)
 (* Well typed store. *)
 Definition STORET (se: stenv) (ss: store)
- := Forall2 (TYPEV nil nil se) ss se.
+ := Forall2 (TYPEB nil nil se) ss se.
 Hint Unfold STORET.
 
 
-(*******************************************************************)
 (* Well formed store. *)
-Definition WfS (se: stenv) (ss: list val)
+Definition WfS (se: stenv) (ss: store)
  := Forall closedT se
  /\ STOREM se ss
  /\ STORET se ss.
 Hint Unfold WfS.
 
-
-(********************************************************************)
-(* When we extend the store and store typing with a new binding, 
-   then the resulting store is still well formed. *)
-Lemma store_extended_wellformed
- :  forall se ss v t
- ,  WfS    se ss
- -> TYPEV  nil nil se v t
- -> WfS    (t <: se) (v <: ss).
-Proof.
- admit.
-Qed.
