devel/Iron/Language/SystemF2Effect/StoreBind.v
@@ -1,0 +1,19 @@
+
+Require Export Iron.Language.SystemF2Effect.Va.
+Require Export Iron.Language.SystemF2Effect.TyJudge.
+Require Export Iron.Language.SystemF2Effect.TyEnv.
+
+
+(* Store bindings are the primitive objects we keep in the store.
+   Each one is tagged with the number of the region is in. *)
+Inductive sbind :=
+ | SBind : nat -> val -> sbind.
+Hint Constructors sbind.
+
+
+(* Types of store bindings. *)
+Inductive TYPEB : kienv -> tyenv -> stenv -> sbind -> ty -> Prop := 
+ | TbBind 
+   :  forall ke te se n v t
+   ,  TYPEV ke te se v t
+   -> TYPEB ke te se (SBind n v) (tRef (TCon (TyConRegion n)) t).
