devel/Iron/Language/SystemF2Effect/VaExpSubst.v
@@ -15,16 +15,16 @@ Fixpoint substTV (d: nat) (u: ty) (vv: val) : val :=
   end
  with    substTX (d: nat) (u: ty) (xx: exp) : exp :=
   match xx with
-  | XVal v       => XVal   (substTV d u v)
-  | XLet t x1 x2 => XLet   (substTT d u t)  (substTX d u x1) (substTX d u x2)
-  | XApp v1 v2   => XApp   (substTV d u v1) (substTV d u v2)
-  | XAPP v1 t2   => XAPP   (substTV d u v1) (substTT d u t2)
+  | XVal v         => XVal   (substTV d u v)
+  | XLet t x1 x2   => XLet   (substTT d u t)  (substTX d u x1) (substTX d u x2)
+  | XApp v1 v2     => XApp   (substTV d u v1) (substTV d u v2)
+  | XAPP v1 t2     => XAPP   (substTV d u v1) (substTT d u t2)
 
-  | XAlloc t1 v2 => XAlloc (substTT d u t1) (substTV d u v2)
-  | XRead  v1    => XRead  (substTV d u v1)
-  | XWrite v1 v2 => XWrite (substTV d u v1) (substTV d u v2)
+  | XAlloc r v     => XAlloc (substTT d u r) (substTV d u v)
+  | XRead  r v     => XRead  (substTT d u r) (substTV d u v)
+  | XWrite r v1 v2 => XWrite (substTT d u r) (substTV d u v1) (substTV d u v2)
 
-  | XOp1 op1 v   => XOp1   op1 (substTV d u v)
+  | XOp1 op1 v     => XOp1   op1 (substTV d u v)
   end.  
 
 
@@ -66,9 +66,9 @@ Fixpoint substVV (d: nat) (u: val) (vv: val) : val :=
   |  XApp v1 v2   => XApp   (substVV d u v1) (substVV d u v2)
   |  XAPP v1 t2   => XAPP   (substVV d u v1) t2
 
-  |  XAlloc t1 v2 => XAlloc t1 (substVV d u v2)
-  |  XRead  v1    => XRead  (substVV d u v1)
-  |  XWrite v1 v2 => XWrite (substVV d u v1) (substVV d u v2)
+  |  XAlloc tR v2    => XAlloc tR (substVV d u v2)
+  |  XRead  tR v1    => XRead  tR (substVV d u v1)
+  |  XWrite tR v1 v2 => XWrite tR (substVV d u v1) (substVV d u v2)
 
   |  XOp1 op v1   => XOp1 op (substVV d u v1)
   end.
